rules/rules_elimination.v
@@ -1,0 +1,86 @@
+(*
+
+  Copyright 2014 Cornell University
+  Copyright 2015 Cornell University
+  Copyright 2016 Cornell University
+  Copyright 2017 Cornell University
+
+  This file is part of VPrl (the Verified Nuprl project).
+
+  VPrl is free software: you can redistribute it and/or modify
+  it under the terms of the GNU General Public License as published by
+  the Free Software Foundation, either version 3 of the License, or
+  (at your option) any later version.
+
+  VPrl is distributed in the hope that it will be useful,
+  but WITHOUT ANY WARRANTY; without even the implied warranty of
+  MERCHANTABILITY or FITNESS FOR A PARTICULAR PURPOSE.  See the
+  GNU General Public License for more details.
+
+  You should have received a copy of the GNU General Public License
+  along with VPrl.  If not, see <http://www.gnu.org/licenses/>.
+
+
+  Websites: http://nuprl.org/html/verification/
+            http://nuprl.org/html/Nuprl2Coq
+            https://github.com/vrahli/NuprlInCoq
+
+  Authors: Abhishek Anand & Vincent Rahli
+
+*)
+
+
+Require Export sequents2.
+Require Export sequents_lib.
+Require Export sequents_tacs.
+Require Export sequents_tacs2.
+Require Export sequents_equality.
+Require Export rules_useful.
+Require Export per_props_equality.
+Require Export per_props_isect.
+Require Export rules_tyfam.
+Require Export rules_tyfam2.
+Require Export subst_tacs_aeq.
+Require Export cequiv_tacs.
+Require Export lsubstc_weak.
+
+Hint Rewrite @nh_vars_hyps_app : slow.
+Hint Rewrite @nh_vars_hyps_snoc : slow.
+
+
+(*
+
+  Our elimination rules are simpler than the ones in Nuprl.
+  This rule is to get back the same behavior
+
+<<
+   H, x : t in T |- C ext e[z\t]
+
+     By elimination z
+
+     H, z : T, x = z = t in T |- e
+>>
+
+ *)
+
+
+Definition rule_elimination_concl {o} (H : @bhyps o) x z t T C e :=
+  mk_baresequent
+    (snoc H (mk_hyp x (mk_member t T)))
+    (mk_concl C (subst e z t)).
+
+Definition rule_elimination_hyp1 {o} (H : @bhyps o) x z t T C e :=
+  mk_baresequent
+    (snoc (snoc H (mk_hyp z T)) (mk_hyp x (mk_equality (mk_var z) t T)))
+    (mk_concl C e).
+
+Definition rule_elimination {o}
+           (H : @bhyps o)
+           (x z : NVar)
+           (t T C e : NTerm) :=
+  mk_rule
+    (rule_elimination_concl H x z t T C e)
+    [
+      rule_elimination_hyp1 H x z t T C e
+    ]
+    [(*sarg_term a, sarg_var z*)].
