rules/rules_isect.v
@@ -32,3 +32,4 @@
 
 Require Export rules_isect_equality.
 Require Export rules_isect_member_formation.
+Require Export rules_isect_elimination.
