rules/rules_isect_equality.v
@@ -1,0 +1,411 @@
+(*
+
+  Copyright 2014 Cornell University
+  Copyright 2015 Cornell University
+  Copyright 2016 Cornell University
+  Copyright 2017 Cornell University
+
+  This file is part of VPrl (the Verified Nuprl project).
+
+  VPrl is free software: you can redistribute it and/or modify
+  it under the terms of the GNU General Public License as published by
+  the Free Software Foundation, either version 3 of the License, or
+  (at your option) any later version.
+
+  VPrl is distributed in the hope that it will be useful,
+  but WITHOUT ANY WARRANTY; without even the implied warranty of
+  MERCHANTABILITY or FITNESS FOR A PARTICULAR PURPOSE.  See the
+  GNU General Public License for more details.
+
+  You should have received a copy of the GNU General Public License
+  along with VPrl.  If not, see <http://www.gnu.org/licenses/>.
+
+
+  Websites: http://nuprl.org/html/verification/
+            http://nuprl.org/html/Nuprl2Coq
+            https://github.com/vrahli/NuprlInCoq
+
+  Authors: Abhishek Anand & Vincent Rahli
+
+*)
+
+
+Require Export sequents2.
+Require Export sequents_lib.
+Require Export sequents_tacs.
+Require Export sequents_tacs2.
+Require Export per_props_equality.
+Require Export per_props_isect.
+Require Export rules_tyfam.
+Require Export rules_tyfam2.
+Require Export subst_tacs_aeq.
+Require Export cequiv_tacs.
+
+
+
+(* end hide *)
+
+(* [8] ============ ISECT EQUALITY ============ *)
+
+(**
+
+  We can state the intersection equality rule as follows:
+<<
+   H |- isect x1:a1. b1 = isect x2:a2.b2 in Type(i)
+
+     By isectEquality y ()
+
+     H |- a1 = a2 in Type(i)
+     H y : a1 |- subst b1 x1 y = subst b2 x2 y in Type(i)
+>>
+ *)
+
+Definition rule_isect_equality_concl {o} a1 a2 x1 x2 b1 b2 i (H : @bhyps o) :=
+  mk_baresequent
+    H
+    (mk_concleq
+       (mk_isect a1 x1 b1)
+       (mk_isect a2 x2 b2)
+       (mk_uni i)).
+
+Definition rule_isect_equality_hyp1 {o} a1 a2 i (H : @bhyps o) :=
+  mk_baresequent H (mk_concleq a1 a2 (mk_uni i)).
+
+Definition rule_isect_equality_hyp2 {o} a1 b1 b2 x1 x2 y i (H : @bhyps o) :=
+  mk_baresequent
+    (snoc H (mk_hyp y a1))
+    (mk_concleq
+       (subst b1 x1 (mk_var y))
+       (subst b2 x2 (mk_var y))
+       (mk_uni i)).
+
+Definition rule_isect_equality {o}
+           (a1 a2 b1 b2 : NTerm)
+           (x1 x2 y : NVar)
+           (i   : nat)
+           (H   : @barehypotheses o) :=
+  mk_rule
+    (rule_isect_equality_concl a1 a2 x1 x2 b1 b2 i H)
+    [ rule_isect_equality_hyp1 a1 a2 i H,
+      rule_isect_equality_hyp2 a1 b1 b2 x1 x2 y i H
+    ]
+    [ sarg_var y ].
+
+Lemma rule_isect_equality_true3 {o} :
+  forall lib (a1 a2 b1 b2 : NTerm),
+  forall x1 x2 y : NVar,
+  forall i   : nat,
+  forall H   : @barehypotheses o,
+    rule_true3 lib (rule_isect_equality
+                      a1 a2 b1 b2
+                      x1 x2 y
+                      i
+                      H).
+Proof.
+  intros.
+  apply (rule_tyfam_equality_true3 _ _ mkc_isect); auto.
+
+  - introv; simpl; allrw remove_nvars_nil_l; allrw app_nil_r; auto.
+
+  - introv; apply lsubstc_mk_isect_ex.
+
+  - introv; apply equality_isect.
+Qed.
+
+Lemma rule_isect_equality_true_ext_lib {o} :
+  forall lib (a1 a2 b1 b2 : NTerm),
+  forall x1 x2 y : NVar,
+  forall i   : nat,
+  forall H   : @barehypotheses o,
+    rule_true_ext_lib lib (rule_isect_equality
+                             a1 a2 b1 b2
+                             x1 x2 y
+                             i
+                             H).
+Proof.
+  introv.
+  apply rule_true3_implies_rule_true_ext_lib.
+  introv.
+  apply rule_isect_equality_true3.
+Qed.
+
+Lemma rule_isect_equality_true {o} :
+  forall lib (a1 a2 b1 b2 : NTerm),
+  forall x1 x2 y : NVar,
+  forall i   : nat,
+  forall H   : @barehypotheses o,
+    rule_true lib (rule_isect_equality
+                     a1 a2 b1 b2
+                     x1 x2 y
+                     i
+                     H).
+Proof.
+  introv.
+  apply rule_true3_implies_rule_true.
+  apply rule_isect_equality_true3.
+Qed.
+
+(* begin hide *)
+
+Lemma rule_isect_equality_true_ex {o} :
+  forall lib y i a1 a2 b1 b2 x1 x2 H,
+    @rule_true_if o lib (rule_isect_equality a1 a2 b1 b2 x1 x2 y i H).
+Proof.
+  intros.
+  generalize (rule_isect_equality_true lib a1 a2 b1 b2 x1 x2 y i H); intro rt.
+  rw <- @rule_true_eq_ex in rt.
+  unfold rule_true_ex in rt; sp.
+Qed.
+
+Lemma rule_isect_equality_true2 {o} :
+  forall lib (y : NVar),
+  forall i : nat,
+  forall a1 a2 b1 b2 : NTerm,
+  forall x1 x2 : NVar,
+  forall H   : @barehypotheses o,
+    rule_true2 lib (rule_isect_equality
+                  a1 a2 b1 b2
+                  x1 x2 y
+                  i
+                  H).
+Proof.
+  introv.
+  apply rule_true_iff_rule_true2; auto.
+  apply rule_isect_equality_true; auto.
+Qed.
+
+Lemma rule_isect_equality_wf {o} :
+  forall y : NVar,
+  forall i : nat,
+  forall a1 a2 b1 b2 : NTerm,
+  forall x1 x2 : NVar,
+  forall H   : @barehypotheses o,
+  forall c1  : !LIn y (vars_hyps H),
+    wf_rule (rule_isect_equality
+               a1 a2 b1 b2
+               x1 x2 y
+               i
+               H).
+Proof.
+  introv c1.
+  introv pwf m.
+
+  allsimpl; repdors; sp; subst; allunfold @pwf_sequent; wfseq;
+  allapply @wf_isect_iff; repnd; auto;
+  allrw @covered_isect; repnd; auto;
+  try (apply subst_preserves_wf_term; auto);
+  try (apply @covered_subst; try (apply @covered_var; rw in_snoc; sp));
+  try (complete (rw cons_snoc; apply @covered_snoc_weak; auto)).
+
+  allrw @vswf_hypotheses_nil_eq.
+  apply wf_hypotheses_snoc; simpl; dands; auto.
+  apply isprog_vars_eq; dands; auto.
+  apply nt_wf_eq; auto.
+Qed.
+
+Lemma rule_isect_equality_wf2 {o} :
+  forall y : NVar,
+  forall i : nat,
+  forall a1 a2 b1 b2 : NTerm,
+  forall x1 x2 : NVar,
+  forall H   : @barehypotheses o,
+  forall c1  : !LIn y (vars_hyps H),
+    wf_rule2 (rule_isect_equality
+                a1 a2 b1 b2
+                x1 x2 y
+                i
+                H).
+Proof.
+  introv c1 pwf m.
+
+  allsimpl; repdors; sp; subst; allunfold @wf_bseq; wfseq;
+  allapply @wf_isect_iff; repnd; auto;
+  allrw @covered_isect; repnd; auto;
+  try (apply subst_preserves_wf_term; auto);
+  try (apply @covered_subst; try (apply @covered_var; rw in_snoc; sp));
+  try (complete (rw cons_snoc; apply @covered_snoc_weak; auto)).
+
+  allrw @vswf_hypotheses_nil_eq.
+  apply wf_hypotheses_snoc; simpl; dands; auto.
+  apply isprog_vars_eq; dands; auto.
+  apply nt_wf_eq; auto.
+Qed.
+
+
+(* Another version that doesn't force the subgoals to have a given extract (axiom here) *)
+
+Definition rule_isect_equality2_hyp1 {o} a1 a2 e1 i (H : @bhyps o) :=
+  mk_baresequent H (mk_concl (mk_equality a1 a2 (mk_uni i)) e1).
+
+Definition rule_isect_equality2_hyp2 {o} a1 b1 b2 e2 x1 x2 y i (H : @bhyps o) :=
+  mk_baresequent
+    (snoc H (mk_hyp y a1))
+    (mk_concl
+       (mk_equality
+          (subst b1 x1 (mk_var y))
+          (subst b2 x2 (mk_var y))
+          (mk_uni i))
+       e2).
+
+Definition rule_isect_equality2 {o}
+           (a1 a2 b1 b2 : @NTerm o)
+           (e1 e2 : NTerm)
+           (x1 x2 y : NVar)
+           (i   : nat)
+           (H   : barehypotheses) :=
+  mk_rule
+    (rule_isect_equality_concl a1 a2 x1 x2 b1 b2 i H)
+    [ rule_isect_equality2_hyp1 a1 a2 e1 i H,
+      rule_isect_equality2_hyp2 a1 b1 b2 e2 x1 x2 y i H
+    ]
+    [ sarg_var y ].
+
+Lemma rule_isect_equality2_true3 {o} :
+  forall lib (a1 a2 b1 b2 : NTerm) e1 e2,
+  forall x1 x2 y : NVar,
+  forall i   : nat,
+  forall H   : @barehypotheses o,
+    rule_true3 lib (rule_isect_equality2
+                      a1 a2 b1 b2
+                      e1 e2
+                      x1 x2 y
+                      i
+                      H).
+Proof.
+  intros.
+  apply (rule_tyfam_equality2_true3 _ _ mkc_isect); auto.
+
+  - introv; simpl; allrw remove_nvars_nil_l; allrw app_nil_r; auto.
+
+  - introv; apply lsubstc_mk_isect_ex.
+
+  - introv; apply equality_isect.
+Qed.
+
+Lemma rule_isect_equality2_true_ext_lib {o} :
+  forall lib (a1 a2 b1 b2 : NTerm) e1 e2,
+  forall x1 x2 y : NVar,
+  forall i   : nat,
+  forall H   : @barehypotheses o,
+    rule_true_ext_lib lib (rule_isect_equality2
+                             a1 a2 b1 b2
+                             e1 e2
+                             x1 x2 y
+                             i
+                             H).
+Proof.
+  introv.
+  apply rule_true3_implies_rule_true_ext_lib.
+  introv.
+  apply rule_isect_equality2_true3.
+Qed.
+
+Lemma rule_isect_equality2_true {o} :
+  forall lib (a1 a2 b1 b2 : NTerm) e1 e2,
+  forall x1 x2 y : NVar,
+  forall i   : nat,
+  forall H   : @barehypotheses o,
+    rule_true lib (rule_isect_equality2
+                     a1 a2 b1 b2
+                     e1 e2
+                     x1 x2 y
+                     i
+                     H).
+Proof.
+  introv.
+  apply rule_true3_implies_rule_true.
+  apply rule_isect_equality2_true3.
+Qed.
+
+Lemma rule_isect_equality2_true_ex {o} :
+  forall lib y i a1 a2 b1 b2 e1 e2 x1 x2 H,
+    @rule_true_if o lib (rule_isect_equality2 a1 a2 b1 b2 e1 e2 x1 x2 y i H).
+Proof.
+  intros.
+  generalize (rule_isect_equality2_true lib a1 a2 b1 b2 e1 e2 x1 x2 y i H); intro rt.
+  rw <- @rule_true_eq_ex in rt.
+  unfold rule_true_ex in rt; sp.
+Qed.
+
+Lemma rule_isect_equality2_true2 {o} :
+  forall lib (y : NVar),
+  forall i : nat,
+  forall a1 a2 b1 b2 : NTerm,
+  forall e1 e2,
+  forall x1 x2 : NVar,
+  forall H   : @barehypotheses o,
+    rule_true2 lib (rule_isect_equality2
+                      a1 a2 b1 b2
+                      e1 e2
+                      x1 x2 y
+                      i
+                      H).
+Proof.
+  introv.
+  apply rule_true_iff_rule_true2; auto.
+  apply rule_isect_equality2_true; auto.
+Qed.
+
+Lemma rule_isect_equality2_wf {o} :
+  forall y : NVar,
+  forall i : nat,
+  forall a1 a2 b1 b2 : NTerm,
+  forall e1 e2,
+  forall x1 x2 : NVar,
+  forall H   : @barehypotheses o,
+  forall c1  : !LIn y (vars_hyps H),
+  forall w1  : wf_term e1,
+  forall w2  : wf_term e2,
+    wf_rule (rule_isect_equality2
+               a1 a2 b1 b2
+               e1 e2
+               x1 x2 y
+               i
+               H).
+Proof.
+  introv c1 w1 w2 pwf m.
+
+  allsimpl; repdors; sp; subst; allunfold @pwf_sequent; wfseq;
+  allapply @wf_isect_iff; repnd; auto;
+  allrw @covered_isect; repnd; auto;
+  try (apply subst_preserves_wf_term; auto);
+  try (apply @covered_subst; try (apply @covered_var; rw in_snoc; sp));
+  try (complete (rw cons_snoc; apply @covered_snoc_weak; auto)).
+
+  allrw @vswf_hypotheses_nil_eq.
+  apply wf_hypotheses_snoc; simpl; dands; auto.
+  apply isprog_vars_eq; dands; auto.
+  apply nt_wf_eq; auto.
+Qed.
+
+Lemma rule_isect_equality2_wf2 {o} :
+  forall y : NVar,
+  forall i : nat,
+  forall a1 a2 b1 b2 : NTerm,
+  forall e1 e2,
+  forall x1 x2 : NVar,
+  forall H   : @barehypotheses o,
+  forall c1  : !LIn y (vars_hyps H),
+    wf_rule2 (rule_isect_equality2
+                a1 a2 b1 b2
+                e1 e2
+                x1 x2 y
+                i
+                H).
+Proof.
+  introv c1 pwf m.
+
+  allsimpl; repdors; sp; subst; allunfold @wf_bseq; wfseq;
+  allapply @wf_isect_iff; repnd; auto;
+  allrw @covered_isect; repnd; auto;
+  try (apply subst_preserves_wf_term; auto);
+  try (apply @covered_subst; try (apply @covered_var; rw in_snoc; sp));
+  try (complete (rw cons_snoc; apply @covered_snoc_weak; auto)).
+
+  allrw @vswf_hypotheses_nil_eq.
+  apply wf_hypotheses_snoc; simpl; dands; auto.
+  apply isprog_vars_eq; dands; auto.
+  apply nt_wf_eq; auto.
+Qed.
+
+(* end hide *)
