rules/rules_isect_member_formation.v
@@ -1,0 +1,392 @@
+(*
+
+  Copyright 2014 Cornell University
+  Copyright 2015 Cornell University
+  Copyright 2016 Cornell University
+  Copyright 2017 Cornell University
+
+  This file is part of VPrl (the Verified Nuprl project).
+
+  VPrl is free software: you can redistribute it and/or modify
+  it under the terms of the GNU General Public License as published by
+  the Free Software Foundation, either version 3 of the License, or
+  (at your option) any later version.
+
+  VPrl is distributed in the hope that it will be useful,
+  but WITHOUT ANY WARRANTY; without even the implied warranty of
+  MERCHANTABILITY or FITNESS FOR A PARTICULAR PURPOSE.  See the
+  GNU General Public License for more details.
+
+  You should have received a copy of the GNU General Public License
+  along with VPrl.  If not, see <http://www.gnu.org/licenses/>.
+
+
+  Websites: http://nuprl.org/html/verification/
+            http://nuprl.org/html/Nuprl2Coq
+            https://github.com/vrahli/NuprlInCoq
+
+  Authors: Abhishek Anand & Vincent Rahli
+
+*)
+
+
+Require Export sequents2.
+Require Export sequents_lib.
+Require Export sequents_tacs.
+Require Export sequents_tacs2.
+Require Export per_props_equality.
+Require Export per_props_isect.
+Require Export rules_tyfam.
+Require Export rules_tyfam2.
+Require Export subst_tacs_aeq.
+Require Export cequiv_tacs.
+
+
+
+(* end hide *)
+
+(**
+
+  We now prove the truth of several rules about the intersection type.
+
+*)
+
+(* [3] ============ ISECT MEMBER FORMATION ============ *)
+
+(**
+
+  We can state the intersection member formation rule as follows:
+
+<<
+   H |- isect x:A. B ext b
+
+     By isect_memberFormation lvl(i) z ()
+
+     H [z : A] |- subst B x z ext b
+     H |- A = A in Type(i)
+>>
+
+ *)
+
+Definition rule_isect_member_formation_concl {o} A x B b (H : @bhyps o) :=
+  mk_baresequent H (mk_concl (mk_isect A x B) b).
+
+Definition rule_isect_member_formation_hyp1 {o} z A x B b (H : @bhyps o) :=
+  mk_baresequent
+    (snoc H (mk_hhyp z A))
+    (mk_concl (subst B x (mk_var z)) b).
+
+Definition rule_isect_member_formation_hyp2 {o} A e i (H : @bhyps o) :=
+  mk_baresequent H (mk_concl (mk_equality A A (mk_uni i)) e).
+
+Definition rule_isect_member_formation {o}
+           (A B b e : NTerm)
+           (x z  : NVar)
+           (i    : nat)
+           (H    : @barehypotheses o) :=
+  mk_rule
+    (rule_isect_member_formation_concl A x B b H)
+    [ rule_isect_member_formation_hyp1 z A x B b H,
+      rule_isect_member_formation_hyp2 A e i H ]
+    [sarg_var z].
+
+Lemma rule_isect_member_formation_true3 {o} :
+  forall lib (A B b e : NTerm)
+         (x z : NVar)
+         (i   : nat)
+         (H   : @barehypotheses o),
+    rule_true3 lib (rule_isect_member_formation A B b e x z i H).
+Proof.
+  intros.
+  unfold rule_isect_member_formation, rule_true3, wf_bseq, closed_type_baresequent, closed_extract_baresequent; simpl.
+  intros; repnd.
+
+  (* We prove the well-formedness of things *)
+  destseq; allsimpl.
+  dLin_hyp; exrepnd.
+  rename Hyp into hyp1.
+  rename Hyp0 into hyp2.
+  destruct hyp1 as [ ws1 hyp1 ].
+  destruct hyp2 as [ ws2 hyp2 ].
+  destseq; allsimpl; proof_irr; GC.
+
+  assert (wf_csequent ((H) ||- (mk_concl (mk_isect A x B) b))) as wfc.
+  { clear hyp1 hyp2.
+    unfold wf_csequent, closed_type, closed_extract, wf_sequent, wf_concl; simpl.
+    dwfseq.
+    rw @vswf_hypotheses_nil_eq.
+    dands; auto.
+    introv j.
+    rw in_app_iff in j; repndors; tcsp.
+  }
+
+  exists wfc.
+  unfold wf_csequent, wf_sequent, wf_concl in wfc; allsimpl; repnd; proof_irr; GC.
+
+  (* We prove some simple facts on our sequents *)
+  assert (covered b (nh_vars_hyps H)
+          # (z <> x -> !LIn z (free_vars B))
+          # !LIn z (free_vars b)
+          # !LIn z (free_vars A)
+          # !LIn z (vars_hyps H)
+          # @wf_term o (mk_var z)) as vhyps.
+
+  { clear hyp1 hyp2.
+    dwfseq.
+    sp;
+      try (complete (generalize (wfc1 z); sp;
+                     allrw in_remove_nvars; allsimpl;
+                     autodimp X0 h; sp));
+      try (complete (apply_in_hyp p;
+                     generalize (subvars_hs_vars_hyps H); intro sv;
+                     rw subvars_prop in sv;
+                     apply sv in p; sp)).
+  }
+
+  destruct vhyps as [ bcH vhyps ].
+  destruct vhyps as [ nzB vhyps ].
+  destruct vhyps as [ nzb vhyps ].
+  destruct vhyps as [ nzA vhyps ].
+  destruct vhyps as [ nzH wfz ].
+  (* done with proving these simple facts *)
+
+  (* we now start proving the sequent *)
+  vr_seq_true.
+
+  (* We prove our first subgoal *)
+  assert (forall s2 pC2,
+            similarity lib s1 s2 H
+            -> tequality lib (lsubstc (mk_isect A x B) wf1 s1 pC1)
+                         (lsubstc (mk_isect A x B) wf1 s2 pC2)) as tfb.
+
+  { clear s2 pC2 pt2 sim.
+    intros s2 pC2 sim.
+    lift_lsubst.
+    rw @tequality_isect.
+
+    (* we have to prove that A is a type and B is a type family *)
+    split.
+
+    - (* we use our 2nd hypothesis to prove that A is a type *)
+      vr_seq_true in hyp2.
+      generalize (hyp2 s1 s2); clear hyp2; intro hyp2.
+      autodimp hyp2 h.
+      autodimp hyp2 h; exrepd.
+      lsubst_tac.
+      apply equality_in_mkc_equality in e0; repnd.
+      clear e0 e2.
+      apply equality_commutes in t; auto.
+      apply equality_in_uni in t; auto.
+
+    - (* we use our 1st hypothesis to prove that B is a type family *)
+      intros.
+      vr_seq_true in hyp1.
+      generalize (hyp1 (snoc s1 (z, a)) (snoc s2 (z, a'))); clear hyp1; intro hyp1.
+      autodimp hyp1 h.
+
+      + (* To use our 1st hyp, we first have to prove that the hypotheses are functional *)
+        intros s3 sim3.
+        inversion sim3; cpx; allsimpl; cpx; clear_irr.
+        assert (cover_vars A s4) as c4
+            by (apply similarity_cover_vars with (t := A) in sim0; auto).
+        (* we use our hyp (coming from proving that our sequent is true) that says that H is functional *)
+        rw @eq_hyps_snoc; simpl.
+
+        exists s1 s4 a t2 w1 c1 c4; sp.
+        (* now to prove that functionality statement on A, we use our 2nd hyp *)
+        vr_seq_true in hyp2.
+        generalize (hyp2 s1 s4); clear hyp2; intro hyp2.
+        autodimp hyp2 hyp.
+        autodimp hyp2 hyp; exrepd.
+        lsubst_tac.
+        apply equality_in_mkc_equality in e1; repnd.
+        clear e1 e3.
+        apply equality_commutes in t; auto.
+        apply equality_in_uni in t; auto.
+        (* and we're done proving that the hypotheses are functional *)
+
+      + (* now we can keep using our 1st hypothesis *)
+        autodimp hyp1 hyp.
+
+        { (* For that we have to prove that the two terms we picked to be equal in A are actually equal in A *)
+          sim_snoc; dands; auto. }
+
+        { (* and again, we keep on using our 1st hypothesis *)
+          exrepd. (* we prove that from t *)
+
+          assert (cover_vars (mk_var z) (snoc s1 (z, a))) as cov1.
+          { apply cover_vars_var; rw @dom_csub_snoc; simpl; rw in_snoc; sp. }
+
+          assert (cover_vars (mk_var z) (snoc s2 (z, a'))) as cov2.
+          { apply cover_vars_var; rw @dom_csub_snoc; simpl; rw in_snoc; sp. }
+
+          repeat (lsubstc_subst_aeq2;[]).
+          repeat (substc_lsubstc_vars3;[]).
+          revert c c4 t.
+          lsubst_tac.
+          introv t.
+          repeat (lsubstc_snoc2;[]).
+          proof_irr; auto.
+          (* and we're done proving our 1st subgoal (the tequality) *)
+        }
+  }
+
+  (* We now prove our second subgoal *)
+  dands; auto.
+  lsubst_tac_c.
+  applydup @similarity_refl in sim.
+  rw @equality_in_isect.
+
+  dands.
+  (* We have to prove 3 goals *)
+
+  { (* 1) we have to prove that A is a type *)
+    generalize (tfb s1 pC1 sim0); sp.
+    lsubst_tac.
+    allrw @tequality_isect; sp. }
+
+  { (* 2) we have to prove that B is a type family *)
+    generalize (tfb s1 pC1 sim0); sp.
+    lsubst_tac.
+    allrw @tequality_isect; sp. }
+
+  { (* 3) we have to prove that b is a member B *)
+    introv equ.
+    vr_seq_true in hyp1.
+    generalize (hyp1 (snoc s1 (z, a)) (snoc s2 (z, a'))); clear hyp1; intro hyp1.
+    autodimp hyp1 hyp.
+
+    - (* first we have to prove that the hypotheses are functional *)
+      intros s3 sim3.
+      inversion sim3; cpx; allsimpl; cpx; clear_irr.
+      assert (cover_vars A s4) as c4
+          by (apply @similarity_cover_vars with (t := A) in sim1; auto).
+      (* we use our hyp (coming from proving that our sequent is true) that says that H is functional *)
+      allapplydup eqh.
+      rw @eq_hyps_snoc; simpl.
+      exists s1 s4 a t2 w1 c1 c4; sp.
+      (* now to prove that functionality statement on A, we use our 2nd hyp (from tfb) *)
+      assert (cover_vars (mk_isect A x B) s4) as c5.
+      { eapply similarity_cover_vars; eauto. }
+      pose proof (tfb s4 c5 sim1) as hh.
+      lsubst_tac.
+      allrw @tequality_isect; sp.
+      (* and we're done proving that the hypotheses are functional *)
+
+    - (* now we can keep using our 1st hypothesis *)
+      autodimp hyp1 hyp.
+
+      + (* For that we have to prove that the two terms we picked to be equal in A are actually equal in A *)
+        sim_snoc; dands; auto.
+        (* easy enough *)
+
+      + (* and again, we keep on using our 1st hypothesis *)
+        exrepd. (* we prove that from e *)
+        clear t; clear_irr.
+
+        assert (cover_vars (mk_var z) (snoc s1 (z, a))) as cov1.
+        { apply cover_vars_var; rw @dom_csub_snoc; simpl; rw in_snoc; sp. }
+
+        lsubstc_subst_aeq2.
+        repeat (substc_lsubstc_vars3;[]).
+        revert c0 e0.
+        lsubst_tac.
+        introv e0.
+        lsubstc_snoc2.
+        proof_irr; auto.
+  }
+Qed.
+
+Lemma rule_isect_member_formation_true_ext_lib {o} :
+  forall lib (A B b e : NTerm)
+         (x z : NVar)
+         (i   : nat)
+         (H   : @barehypotheses o),
+    rule_true_ext_lib lib (rule_isect_member_formation A B b e x z i H).
+Proof.
+  introv.
+  apply rule_true3_implies_rule_true_ext_lib.
+  introv.
+  apply rule_isect_member_formation_true3.
+Qed.
+
+
+(* begin hide *)
+
+Lemma rule_isect_member_formation_true {o} :
+  forall lib (A B b e : NTerm)
+         (x z : NVar)
+         (i   : nat)
+         (H   : @barehypotheses o),
+    rule_true lib (rule_isect_member_formation A B b e x z i H).
+Proof.
+  introv.
+  apply rule_true3_implies_rule_true.
+  apply rule_isect_member_formation_true3.
+Qed.
+
+Lemma rule_isect_member_formation_true_ex {o} :
+  forall lib i z e A B b x H,
+    @rule_true_if o lib (rule_isect_member_formation A B b e x z i H).
+Proof.
+  intros.
+  generalize (rule_isect_member_formation_true lib A B b e x z i H); intro rt.
+  rw <- @rule_true_eq_ex in rt.
+  unfold rule_true_ex in rt; sp.
+Qed.
+
+Lemma rule_isect_member_formation_true2 {o} :
+  forall lib i z e A B b x H,
+    @rule_true2 o lib (rule_isect_member_formation A B b e x z i H).
+Proof.
+  intros.
+  generalize (rule_isect_member_formation_true lib A B b e x z i H); intro rt.
+  apply rule_true_iff_rule_true2; sp.
+Qed.
+
+Lemma rule_isect_member_formation_wf {o} :
+  forall i z e A B b x H,
+    !LIn z (vars_hyps H)
+    -> wf_term e
+    -> @wf_rule o (rule_isect_member_formation A B b e x z i H).
+Proof.
+  introv niz wfe.
+
+  introv pwf m; allsimpl; repdors; subst; sp;
+    allunfold @pwf_sequent; wfseq; sp;
+      allrw @covered_isect; repnd; auto;
+        allrw <- @wf_isect_iff; repnd; auto.
+
+  { allrw @vswf_hypotheses_nil_eq.
+    apply wf_hypotheses_snoc; simpl; sp.
+    apply isprog_vars_eq; sp.
+    apply nt_wf_eq; sp. }
+
+  { apply subst_preserves_wf_term; sp. }
+
+  { apply @covered_subst; sp;
+      try (apply @covered_var; rw in_snoc; sp);
+      try (complete (rw cons_snoc; apply @covered_snoc_weak; auto)). }
+Qed.
+
+Lemma rule_isect_member_formation_wf2 {o} :
+  forall i z A B b e x H,
+    !LIn z (vars_hyps H)
+    -> @wf_rule2 o (rule_isect_member_formation A B b e x z i H).
+Proof.
+  introv niz wf j; allsimpl; repndors; subst; tcsp;
+    allunfold @wf_bseq; repnd; allsimpl; wfseq;
+      allrw @covered_isect; repnd; auto;
+        allrw <- @wf_isect_iff; repnd; auto.
+
+  - allrw @vswf_hypotheses_nil_eq.
+    apply wf_hypotheses_snoc; simpl; sp.
+    apply isprog_vars_eq; sp.
+    apply nt_wf_eq; sp.
+
+  - apply subst_preserves_wf_term; sp.
+
+  - apply @covered_subst; sp;
+    try (apply @covered_var; rw in_snoc; sp);
+    try (complete (rw cons_snoc; apply @covered_snoc_weak; auto)).
+Qed.
